a middle-level proof for LAS (assuming id_rhs_val is correct).
git-svn-id: https://webdav.seas.upenn.edu/svn/sol/vol@3623 eef5ea85-cc2e-0410-bd84-0fae1f012da8

src/Transforms/las.v
@@ -378,13 +378,27 @@ List.Forall2
        products_simulation pinfo lasinfo Ps1 Ps1
    end) S1 S2.
 
+Definition phis_simulation (pinfo: PhiInfo) (lasinfo: LASInfo pinfo) (f1:fdef)
+  ps1 ps2 : Prop :=
+  if (fdef_dec (PI_f pinfo) f1) then 
+    List.map (subst_phi (LAS_lid pinfo lasinfo) (LAS_value pinfo lasinfo)) ps1 
+      = ps2
+  else ps1 = ps2.
+
+Definition tmn_simulation (pinfo: PhiInfo) (lasinfo: LASInfo pinfo) (f1:fdef)
+  t t': Prop :=
+if (fdef_dec (PI_f pinfo) f1) then 
+  subst_tmn (LAS_lid pinfo lasinfo) (LAS_value pinfo lasinfo) t = t'
+else t = t'.
+
 Definition EC_simulation (pinfo: PhiInfo) (lasinfo: LASInfo pinfo) 
   (EC1 EC2:@Opsem.ExecutionContext DGVs) : Prop :=
   match (EC1, EC2) with
   | (Opsem.mkEC f1 b1 cs1 tmn1 lc1 als1, 
      Opsem.mkEC f2 b2 cs2 tmn2 lc2 als2) =>
        fdef_simulation pinfo lasinfo f1 f2 /\
-       tmn1 = tmn2 /\ als1 = als2 /\
+       tmn_simulation pinfo lasinfo f1 tmn1 tmn2 /\
+       als1 = als2 /\
        block_simulation pinfo lasinfo f1 b1 b2 /\
        (exists l1, exists ps1, exists cs11, 
          b1 = block_intro l1 ps1 (cs11++cs1) tmn1)
@@ -418,20 +432,1091 @@ match (St1, St2) with
     gl1 = gl2 /\ fs1 = fs2 /\ M1 = M2
 end.
 
+Lemma cmds_simulation_nil_inv: forall pinfo lasinfo f1 cs,
+  cmds_simulation pinfo lasinfo f1 nil cs -> cs = nil.
+Proof.
+  unfold cmds_simulation. simpl.
+  intros. destruct (fdef_dec (PI_f pinfo) f1); auto.
+Qed.
+
+Definition cmd_simulation (pinfo: PhiInfo) (lasinfo: LASInfo pinfo) (f1:fdef)
+  c c': Prop :=
+if (fdef_dec (PI_f pinfo) f1) then 
+  subst_cmd (LAS_lid pinfo lasinfo) (LAS_value pinfo lasinfo) c = c'
+else c = c'.
+
+Lemma cmds_simulation_cons_inv: forall pinfo lasinfo F c1 cs2 cs',
+  cmds_simulation pinfo lasinfo F (c1 :: cs2) cs' ->
+  exists c1', exists cs2', 
+    cs' = c1' :: cs2' /\
+    cmd_simulation pinfo lasinfo F c1 c1' /\
+    cmds_simulation pinfo lasinfo F cs2 cs2'.
+Proof.  
+  intros.
+  unfold cmds_simulation, cmd_simulation in *.
+  destruct (fdef_dec (PI_f pinfo) F); subst; simpl; eauto.
+Qed.
+
+Ltac wfCall_inv :=
+match goal with
+| Heq3 : exists _,
+           exists _,
+             exists _,
+               ?B = block_intro _ _ _ _,
+  HBinF1 : blockInFdefB ?B ?F = true,
+  HwfCall : OpsemPP.wf_call 
+              {| 
+              Opsem.CurFunction := ?F;
+              Opsem.CurBB := ?B;
+              Opsem.CurCmds := nil;
+              Opsem.Terminator := _;
+              Opsem.Locals := _;
+              Opsem.Allocas := _ |} 
+              ({|
+               Opsem.CurFunction := _;
+               Opsem.CurBB := _;
+               Opsem.CurCmds := ?c' :: _;
+               Opsem.Terminator := _;
+               Opsem.Locals := _;
+               Opsem.Allocas := _ |}  :: _) |- _ =>
+  destruct Heq3 as [l3 [ps3 [cs3 Heq3]]]; subst;
+  assert (HBinF1':=HBinF1);
+  apply HwfCall in HBinF1';
+  destruct c'; tinv HBinF1'; clear HBinF1'
+end.
+
+Ltac destruct_ctx_return :=
+match goal with
+| Hwfpp : OpsemPP.wf_State
+            {|
+            OpsemAux.CurSystem := _;
+            OpsemAux.CurTargetData := ?TD;
+            OpsemAux.CurProducts := _;
+            OpsemAux.Globals := _;
+            OpsemAux.FunTable := _
+             |} _,
+  HwfS1 : wf_State _ _ _ _ _,
+  Hsim : State_simulation _ _ _ _ ?Cfg2 ?St2 ,
+  Hop2 : Opsem.sInsn _ _ _ _ |- _ =>
+  destruct TD as [los nts];
+  destruct Hwfpp as 
+    [Hwfg [HwfSystem [HmInS [_ [
+     [Hreach1 [HBinF1 [HFinPs1 _]]] 
+     [ _ HwfCall'
+     ]]
+    ]]]]; subst;
+  destruct Cfg2 as [S2 TD2 Ps2 gl2 fs2];
+  destruct St2 as [ECs2 M2];
+  simpl in Hsim;
+  destruct Hsim as [EQ1 [Hpsim [Hstksim [EQ2 [EQ3 EQ4]]]]]; subst;
+  destruct ECs2 as [|[F2 B2 cs2 tmn2 lc2 als2] ECs2]; tinv Hstksim;
+  destruct Hstksim as [Hecsim Hstksim];
+  destruct ECs2 as [|[F3 B3 cs3 tmn3 lc3 als3] ECs2]; tinv Hstksim;
+  destruct Hstksim as [Hecsim' Hstksim];
+  unfold EC_simulation in Hecsim;
+  destruct Hecsim as 
+      [Hfsim2 [Htsim2 [Heq2 [Hbsim2 
+        [Heq3 [Heq4 [Hlcsim2 Hcssim2]]]]]]]; subst;
+  destruct Hecsim' as 
+      [Hfsim2' [Htsim2' [Heq2' [Hbsim2' 
+        [Heq3' [Heq4' [Hlcsim2' Hcssim2']]]]]]]; subst;
+  destruct HwfS1 as [Hinscope1' [Hinscope2' HwfECs']];
+  fold wf_ECStack in HwfECs';
+  unfold wf_ExecutionContext in Hinscope1', Hinscope2';
+  simpl in Hinscope1', Hinscope2';
+  apply cmds_simulation_nil_inv in Hcssim2; subst;
+  apply cmds_simulation_cons_inv in Hcssim2'; 
+  destruct Hcssim2' as [c1' [cs3' [Heq [Hcsim2' Hcssim2']]]]; subst
+end.
+
+Lemma fdef_sim__block_sim : forall pinfo lasinfo f1 f2 b1 b2 l0,
+  fdef_simulation pinfo lasinfo f1 f2 ->
+  lookupBlockViaLabelFromFdef f1 l0 = Some b1 ->
+  lookupBlockViaLabelFromFdef f2 l0 = Some b2 ->
+  block_simulation pinfo lasinfo f1 b1 b2.
+Admitted.
+
+Ltac uniq_result :=
+repeat dgvs_instantiate_inv;
+repeat match goal with
+| H1 : ?f ?a ?b ?c ?d = _,
+  H2 : ?f ?a ?b ?c ?d = _ |- _ =>
+  rewrite H1 in H2; inv H2
+| H1 : ?f ?a ?b ?c = _,
+  H2 : ?f ?a ?b ?c = _ |- _ =>
+  rewrite H1 in H2; inv H2
+| H1 : ?f ?a ?b = _,
+  H2 : ?f ?a ?b = _ |- _ =>
+  rewrite H1 in H2; inv H2
+| H1 : _ @ _ |- _ => inv H1
+end.
+
+Lemma block_simulation_inv : forall pinfo lasinfo F l1 ps1 cs1 tmn1 l2 ps2 cs2
+  tmn2,
+  block_simulation pinfo lasinfo F (block_intro l1 ps1 cs1 tmn1)
+    (block_intro l2 ps2 cs2 tmn2) ->
+  l1 = l2 /\ 
+  phis_simulation pinfo lasinfo F ps1 ps2 /\ 
+  cmds_simulation pinfo lasinfo F cs1 cs2 /\ 
+  tmn_simulation pinfo lasinfo F tmn1 tmn2.
+Proof.
+  intros.
+  unfold block_simulation, cmds_simulation, phis_simulation, tmn_simulation in *.
+  destruct (fdef_dec (PI_f pinfo) F); inv H; auto.
+Qed.
+
+Definition value_simulation (pinfo: PhiInfo) (lasinfo: LASInfo pinfo) (f1:fdef)
+  v v': Prop :=
+if (fdef_dec (PI_f pinfo) f1) then 
+  subst_value (LAS_lid pinfo lasinfo) (LAS_value pinfo lasinfo) v = v'
+else v = v'.
+
+Lemma getOperandValue_inTmnOperands_sim : forall los nts ifs s ps gl pinfo 
+  lasinfo (f : fdef) (Hwfg : wf_global (los,nts) s gl) 
+  (HwfF: wf_fdef ifs s (module_intro los nts ps) f)
+  (tmn : terminator)
+  (lc : GVMap)
+  (l1 : l)
+  (ps1 : phinodes)
+  (cs1 : list cmd)
+  (Hreach : isReachableFromEntry f (block_intro l1 ps1 cs1 tmn))
+  (HbInF : blockInFdefB (block_intro l1 ps1 cs1 tmn) f = true)
+  (l0 : list atom)
+  (HeqR : ret l0 = inscope_of_tmn f (block_intro l1 ps1 cs1 tmn) tmn)
+  (Hinscope : id_rhs_val.wf_defs (value_id (LAS_lid pinfo lasinfo))
+                     (LAS_value pinfo lasinfo) (PI_f pinfo) 
+                     (los, nts) gl f lc l0)
+  (v v' : value)
+  (Hvincs : valueInTmnOperands v tmn) gv gv'
+  (Hget' : getOperandValue (los, nts) v' lc gl = Some gv')
+  (Hvsim : value_simulation pinfo lasinfo f v v')
+  (Hget : getOperandValue (los, nts) v lc gl = Some gv),
+  gv = gv'.
+Proof.
+  intros.
+  unfold value_simulation in Hvsim.
+  unfold wf_defs in Hinscope.
+  destruct (fdef_dec (PI_f pinfo) f); subst; try solve [uniq_result; auto].
+  destruct v; subst; simpl in Hget', Hget, Hinscope;
+    try solve [uniq_result; auto].
+  destruct (id_dec i0 (LAS_lid pinfo lasinfo)); simpl in Hget'; subst;
+    try solve [uniq_result; auto].  
+  eapply Hinscope in Hget; eauto.
+    admit. (* wf *)
+    admit. (* wf + v >> lid *)
+Qed.
+
+Lemma getOperandValue_inCmdOperands_sim : forall los nts ifs s gl pinfo lasinfo
+  ps (f : fdef) (Hwfg : wf_global (los,nts) s gl)
+  (HwfSys1 : wf_system ifs s)
+  (HwfF : wf_fdef ifs s (module_intro los nts ps) f)
+  (tmn : terminator)
+  (lc : GVMap)
+  (l1 : l)
+  (ps1 : phinodes)
+  (cs1 cs : list cmd)
+  (c : cmd)
+  (Hreach : isReachableFromEntry f (block_intro l1 ps1 (cs1 ++ c :: cs) tmn))
+  (HbInF : blockInFdefB (block_intro l1 ps1 (cs1 ++ c :: cs) tmn) f = true)
+  (l0 : list atom)
+  (HeqR : ret l0 = inscope_of_cmd f (block_intro l1 ps1 (cs1 ++ c :: cs) tmn) c)
+  (Hinscope : id_rhs_val.wf_defs (value_id (LAS_lid pinfo lasinfo))
+                     (LAS_value pinfo lasinfo) (PI_f pinfo) 
+                     (los, nts) gl f lc l0)
+  (v v' : value)
+  (Hvincs : valueInCmdOperands v c) gv gv'
+  (Hget' : getOperandValue (los, nts) v' lc gl = Some gv')
+  (Hvsim : value_simulation pinfo lasinfo f v v')
+  (Hget : getOperandValue (los, nts) v lc gl = Some gv),
+  gv = gv'.
+Proof.
+  intros.
+  unfold value_simulation in Hvsim.
+  unfold wf_defs in Hinscope.
+  destruct (fdef_dec (PI_f pinfo) f); subst; try solve [uniq_result; auto].
+  destruct v; subst; simpl in Hget', Hget, Hinscope;
+    try solve [uniq_result; auto].
+  destruct (id_dec i0 (LAS_lid pinfo lasinfo)); simpl in Hget'; subst;
+    try solve [uniq_result; auto].  
+  eapply Hinscope in Hget; eauto.
+    admit. (* wf *)
+    admit. (* wf + v >> lid *)
+Qed.
+
+Lemma phis_simulation_nil_inv: forall pinfo lasinfo f1 ps,
+  phis_simulation pinfo lasinfo f1 nil ps -> ps = nil.
+Proof.
+  unfold phis_simulation. simpl.
+  intros. destruct (fdef_dec (PI_f pinfo) f1); auto.
+Qed.
+
+Definition phi_simulation (pinfo: PhiInfo) (lasinfo: LASInfo pinfo) (f1:fdef)
+  p1 p2 : Prop :=
+  if (fdef_dec (PI_f pinfo) f1) then 
+    subst_phi (LAS_lid pinfo lasinfo) (LAS_value pinfo lasinfo) p1 = p2
+  else p1 = p2.
+
+Lemma phis_simulation_cons_inv: forall pinfo lasinfo F p1 ps2 ps',
+  phis_simulation pinfo lasinfo F (p1 :: ps2) ps' ->
+  exists p1', exists ps2', 
+    ps' = p1' :: ps2' /\
+    phi_simulation pinfo lasinfo F p1 p1' /\
+    phis_simulation pinfo lasinfo F ps2 ps2'.
+Proof.  
+  intros.
+  unfold phis_simulation, phi_simulation in *.
+  destruct (fdef_dec (PI_f pinfo) F); subst; simpl; eauto.
+Qed.
+
+Definition list_value_l_simulation (pinfo: PhiInfo) (lasinfo: LASInfo pinfo) 
+  (f1:fdef) vls vls': Prop :=
+if (fdef_dec (PI_f pinfo) f1) then 
+  subst_list_value_l (LAS_lid pinfo lasinfo) (LAS_value pinfo lasinfo) vls = vls'
+else vls = vls'.
+
+Lemma phi_simulation_inv: forall pinfo lasinfo f1 i1 t1 vls1 i2 t2 vls2,
+  phi_simulation pinfo lasinfo f1 (insn_phi i1 t1 vls1) (insn_phi i2 t2 vls2) ->
+  i1 = i2 /\ t1 = t2 /\ list_value_l_simulation pinfo lasinfo f1 vls1 vls2.
+Proof.
+  unfold phi_simulation, list_value_l_simulation.
+  intros.
+  destruct (fdef_dec (PI_f pinfo) f1); inv H; auto.
+Qed.
+
+Lemma getValueViaLabelFromValuels_sim : forall l1 pinfo lasinfo f1 vls1 vls2 v 
+  v' (Hsim: list_value_l_simulation pinfo lasinfo f1 vls1 vls2)
+  (HeqR0 : ret v = getValueViaLabelFromValuels vls1 l1)
+  (HeqR' : ret v' = getValueViaLabelFromValuels vls2 l1),
+  value_simulation pinfo lasinfo f1 v v'.
+Proof.
+  induction vls1; simpl; intros; try congruence.
+    unfold list_value_l_simulation, value_simulation in *.
+    destruct (fdef_dec (PI_f pinfo) f1); subst.
+      simpl in HeqR'.
+      destruct (l0 == l1); subst; eauto.
+        congruence.
+
+    simpl in HeqR'.
+    destruct (l0 == l1); subst; try (congruence || eauto).
+Qed.
+
+Lemma getValueViaLabelFromValuels_getOperandValue_sim : forall
+  los nts ifs s gl pinfo lasinfo
+  ps (f : fdef) (Hwfg : wf_global (los,nts) s gl)
+  (HwfF : wf_fdef ifs s (module_intro los nts ps) f) (HuniqF: uniqFdef f)
+  (l0 : l) (lc : GVMap) (t : list atom) (l1 : l) (ps1 : phinodes)
+  (cs1 : cmds) (tmn1 : terminator) 
+  (HeqR : ret t = inscope_of_tmn f (block_intro l1 ps1 cs1 tmn1) tmn1)
+  (Hinscope : id_rhs_val.wf_defs (value_id (LAS_lid pinfo lasinfo))
+                     (LAS_value pinfo lasinfo) (PI_f pinfo) 
+                     (los, nts) gl f lc t)
+  (ps' : phinodes) (cs' : cmds) (tmn' : terminator)
+  (i0 : id) (l2 : list_value_l) (ps2 : list phinode)
+  (Hreach : isReachableFromEntry f (block_intro l0 ps' cs' tmn'))
+  (HbInF : blockInFdefB (block_intro l1 ps1 cs1 tmn1) f = true)
+  (Hreach' : isReachableFromEntry f (block_intro l1 ps1 cs1 tmn1))
+  (v0 v0': value)
+  (HeqR3 : ret v0 = getValueViaLabelFromValuels l2 l1)
+  (g1 : GenericValue) 
+  (HeqR4 : ret g1 = getOperandValue (los,nts) v0 lc gl)
+  (g2 : GVMap) (g : GenericValue) (g0 : GVMap) t1
+  (H1 : wf_value_list
+         (make_list_system_module_fdef_value_typ
+            (map_list_value_l
+               (fun (value_ : value) (_ : l) =>
+                (s, module_intro los nts ps, f, value_, t1)) l2)))
+  (H7 : wf_phinode f (block_intro l0 ps' cs' tmn') (insn_phi i0 t1 l2))
+  (Hvsim: value_simulation pinfo lasinfo f v0 v0')
+  (HeqR1 : ret g = getOperandValue (los,nts) v0' lc gl),
+  g1 = g.
+Proof.
+  intros. symmetry_ctx.
+  unfold value_simulation in Hvsim.
+  destruct (fdef_dec (PI_f pinfo) f); subst; try solve [uniq_result; auto].
+  destruct v0 as [vid | vc]; simpl in HeqR1, HeqR4; try congruence.
+  destruct (id_dec vid (LAS_lid pinfo lasinfo)); subst; simpl in HeqR1; 
+    try congruence.
+  destruct H7 as [Hwfops Hwfvls].
+  assert (Hnth:=HeqR3).
+  eapply getValueViaLabelFromValuels__nth_list_value_l in Hnth; eauto.
+  destruct Hnth as [n Hnth].
+  assert (HwfV:=HeqR3).
+  eapply wf_value_list__getValueViaLabelFromValuels__wf_value in HwfV; eauto.
+  eapply wf_phi_operands__elim in Hwfops; eauto.
+  destruct Hwfops as [vb [b1 [Hlkvb [Hlkb1 Hdom]]]].
+  assert (b1 = block_intro l1 ps1 cs1 tmn1) as EQ.
+    clear - Hlkb1 HbInF HwfF HuniqF.
+    apply blockInFdefB_lookupBlockViaLabelFromFdef in HbInF; auto.
+    rewrite HbInF in Hlkb1. inv Hlkb1; auto.
+  subst.
+  clear Hwfvls HwfV Hnth.
+  destruct Hdom as [J3 | J3]; try solve [contradict Hreach; auto].
+  clear Hreach.
+  unfold blockDominates in J3.         
+  destruct vb. assert (HeqR':=HeqR).
+  unfold inscope_of_tmn in HeqR.
+  destruct (PI_f pinfo) as [[f t2 i1 a v] bs].
+  remember ((dom_analyze (fdef_intro (fheader_intro f t2 i1 a v) bs)) !! l1) 
+    as R1.
+  destruct R1.
+  apply fold_left__spec in HeqR.
+  destruct (eq_atom_dec l3 l1); subst.
+  Case "l3=l1".
+    destruct HeqR as [HeqR _].
+    assert (In (LAS_lid pinfo lasinfo) t) as Hid2InScope.
+      clear - HeqR3 HeqR Hlkb1 J3 Hlkvb HbInF HwfF HuniqF.
+      assert (J':=Hlkvb).
+      apply lookupBlockViaIDFromFdef__blockInFdefB in Hlkvb.
+      apply lookupBlockViaLabelFromFdef_inv in Hlkb1; auto. 
+      destruct Hlkb1 as [J1 J2].
+      eapply blockInFdefB_uniq in J2; eauto.
+      destruct J2 as [J2 [J4 J5]]; subst.
+      apply lookupBlockViaIDFromFdef__InGetBlockIDs in J'.
+      simpl in J'.
+      apply HeqR; auto.
+      admit. (* lid cannot be in args *)
+    eapply Hinscope in HeqR1; eauto.
+      admit. (* v >> lid *)
+  
+  Case "l3<>l1".
+    assert (In l3 (ListSet.set_diff eq_atom_dec bs_contents [l1])) as G.
+      destruct J3 as [J3 | J3]; subst; try congruence.
+      apply ListSet.set_diff_intro; auto.
+        simpl. intro JJ. destruct JJ as [JJ | JJ]; auto.
+    assert (
+      lookupBlockViaLabelFromFdef (fdef_intro (fheader_intro f t2 i1 a v) bs) l3 
+        = ret block_intro l3 p c t0) as J1.
+      clear - Hlkvb HwfF HuniqF.
+      apply lookupBlockViaIDFromFdef__blockInFdefB in Hlkvb.
+      apply blockInFdefB_lookupBlockViaLabelFromFdef in Hlkvb; auto.
+    destruct HeqR as [_ [HeqR _]].
+    apply HeqR in J1; auto.
+    assert (In (LAS_lid pinfo lasinfo) t) as Hid2InScope.
+      clear - J1 HeqR Hlkb1 J3 Hlkvb HbInF HwfF HuniqF.
+      apply J1.
+      apply lookupBlockViaIDFromFdef__InGetBlockIDs in Hlkvb; auto.
+    eapply Hinscope in HeqR1; eauto.
+      admit. (* v >> lid *)
+Qed.
+
+Lemma getIncomingValuesForBlockFromPHINodes_sim : forall
+  los nts ifs s gl pinfo lasinfo
+  ps (f : fdef) (Hwfg : wf_global (los,nts) s gl)
+  (HwfF : wf_fdef ifs s (module_intro los nts ps) f) (HuniqF: uniqFdef f)
+  l0
+  (lc : GVMap)
+  (t : list atom)
+  l1 ps1 cs1 tmn1 
+  (HeqR : ret t = inscope_of_tmn f (block_intro l1 ps1 cs1 tmn1) tmn1)
+  (Hinscope : id_rhs_val.wf_defs (value_id (LAS_lid pinfo lasinfo))
+                     (LAS_value pinfo lasinfo) (PI_f pinfo) 
+                     (los, nts) gl f lc t)
+  (ps' : phinodes)
+  (cs' : cmds)
+  (tmn' : terminator)
+  (Hsucc : In l0 (successors_terminator tmn1))
+  (Hreach : isReachableFromEntry f (block_intro l0 ps' cs' tmn'))
+  (Hreach' : isReachableFromEntry f (block_intro l1 ps1 cs1 tmn1))
+  (HbInF : blockInFdefB
+            (block_intro l1 ps1 cs1 tmn1) f = true)
+  (HwfB : wf_block ifs s (module_intro los nts ps) f 
+            (block_intro l1 ps1 cs1 tmn1))
+  B1' 
+  (Hbsim1: block_simulation pinfo lasinfo f (block_intro l1 ps1 cs1 tmn1) B1')  
+  ps2
+  (H8 : wf_phinodes ifs s (module_intro los nts ps) f 
+          (block_intro l0 ps' cs' tmn') ps2)
+  (Hin: exists ps1, ps' = ps1 ++ ps2) RVs RVs' ps2'
+  (Hpsim2: phis_simulation pinfo lasinfo f ps2 ps2')
+  (Hget : @Opsem.getIncomingValuesForBlockFromPHINodes DGVs (los,nts) ps2 
+           (block_intro l1 ps1 cs1 tmn1) gl lc = ret RVs)
+  (Hget' : @Opsem.getIncomingValuesForBlockFromPHINodes DGVs (los,nts)
+             ps2' B1' gl lc = ret RVs'),
+  RVs = RVs'.
+Proof.
+  induction ps2 as [|[]]; intros; simpl in Hget, Hget'.
+    apply phis_simulation_nil_inv in Hpsim2.
+    subst. simpl in Hget'. congruence.    
+
+    apply phis_simulation_cons_inv in Hpsim2.
+    destruct Hpsim2 as [p1' [ps2'0 [Heq [Hpsim1 Hpsim2]]]]; subst.
+    simpl in Hget'. destruct p1'. 
+    apply phi_simulation_inv in Hpsim1.
+    destruct Hpsim1 as [Heq1 [Heq2 Hvlsim1]]; subst.
+    inv_mbind'. 
+    destruct B1'. simpl in HeqR0.
+    apply block_simulation_inv in Hbsim1.
+    destruct Hbsim1 as [Heq [Hpsim1 [Hcssim1 Htsim1]]]; subst.
+    simpl in HeqR3.
+    eapply getValueViaLabelFromValuels_sim in Hvlsim1; eauto.
+    inv H8. 
+    assert (g = g0) as Heq.
+      inv H6.
+      eapply getValueViaLabelFromValuels_getOperandValue_sim with (l0:=l0); 
+        eauto.
+    subst. 
+    eapply IHps2 with (RVs:=l4) in H7; eauto.
+      congruence.
+
+      destruct Hin as [ps3 Hin]. subst.
+      exists (ps3++[insn_phi i1 t1 l2]).
+      simpl_env. auto.
+Qed.
+
+Lemma switchToNewBasicBlock_sim : forall
+  los nts ifs s gl pinfo lasinfo
+  ps (f : fdef) (Hwfg : wf_global (los,nts) s gl)
+  (HwfF : wf_fdef ifs s (module_intro los nts ps) f) (HuniqF: uniqFdef f)
+  l2 (lc : GVMap) (t : list atom) l1 ps1 cs1 tmn1
+  (HeqR : ret t = inscope_of_tmn f (block_intro l1 ps1 cs1 tmn1) tmn1)
+  (Hinscope : id_rhs_val.wf_defs (value_id (LAS_lid pinfo lasinfo))
+                     (LAS_value pinfo lasinfo) (PI_f pinfo) 
+                     (los, nts) gl f lc t)
+  (ps2 : phinodes) (cs2 : cmds) (tmn2 : terminator)
+  (Hsucc : In l2 (successors_terminator tmn1))
+  (Hreach : isReachableFromEntry f (block_intro l2 ps2 cs2 tmn2))
+  (Hreach' : isReachableFromEntry f (block_intro l1 ps1 cs1 tmn1))
+  (HbInF' : blockInFdefB (block_intro l2 ps2 cs2 tmn2) f = true)
+  (HbInF : blockInFdefB (block_intro l1 ps1 cs1 tmn1) f = true)
+  lc0 lc0'
+  (Hget : @Opsem.switchToNewBasicBlock DGVs (los,nts) 
+    (block_intro l2 ps2 cs2 tmn2) 
+    (block_intro l1 ps1 cs1 tmn1) gl lc = ret lc0) B1' B2'
+  (Hbsim1: block_simulation pinfo lasinfo f (block_intro l1 ps1 cs1 tmn1) B1')  
+  (Hbsim2: block_simulation pinfo lasinfo f (block_intro l2 ps2 cs2 tmn2) B2')
+  (Hget' : @Opsem.switchToNewBasicBlock DGVs (los,nts) B2' B1' gl lc = ret lc0'),
+  lc0 = lc0'.
+Proof.
+  intros.
+  assert (HwfB : wf_block ifs s (module_intro los nts ps) f 
+           (block_intro l1 ps1 cs1 tmn1)).
+    apply wf_fdef__blockInFdefB__wf_block; auto.
+  assert (H8 : wf_phinodes ifs s (module_intro los nts ps) f 
+                 (block_intro l2 ps2 cs2 tmn2) ps2).
+    apply wf_fdef__wf_phinodes; auto.
+  unfold Opsem.switchToNewBasicBlock in *.
+  inv_mbind'. app_inv. symmetry_ctx.
+  assert (l3 = l0) as EQ.
+    destruct B2'.
+    apply block_simulation_inv in Hbsim2.
+    destruct Hbsim2 as [J1 [J2 [J3 J4]]]; subst.
+    eapply getIncomingValuesForBlockFromPHINodes_sim; eauto.
+      exists nil. auto.
+  subst. auto.
+Qed.
+
+Ltac destruct_ctx_other :=
+match goal with
+| Hwfpp : OpsemPP.wf_State
+            {|
+            OpsemAux.CurSystem := _;
+            OpsemAux.CurTargetData := ?TD;
+            OpsemAux.CurProducts := _;
+            OpsemAux.Globals := _;
+            OpsemAux.FunTable := _
+             |} _,
+  HwfS1 : wf_State _ _ _ _ _,
+  Hsim : State_simulation _ _ _ _ ?Cfg2 ?St2 ,
+  Hop2 : Opsem.sInsn _ _ _ _ |- _ =>
+  destruct TD as [los nts];
+  destruct Hwfpp as 
+    [Hwfg [HwfSystem [HmInS [_ [
+     [Hreach1 [HBinF1 [HFinPs1 _]]] 
+     [HwfECs Hwfcall]]
+    ]]]]; subst;
+  fold (@OpsemPP.wf_ECStack DGVs) in HwfECs;
+  destruct Cfg2 as [S2 TD2 Ps2 gl2 fs2];
+  destruct St2 as [ECs2 M2];
+  simpl in Hsim;
+  destruct Hsim as [EQ1 [Hpsim [Hstksim [EQ2 [EQ3 EQ4]]]]]; subst;
+  destruct ECs2 as [|[F2 B2 cs2 tmn2 lc2 als2] ECs2]; tinv Hstksim;
+  destruct Hstksim as [Hecsim Hstksim];
+  unfold EC_simulation in Hecsim;
+  destruct Hecsim as 
+      [Hfsim2 [Htsim2 [Heq2 [Hbsim2 
+        [[l3 [ps3 [cs31 Heq3]]]
+        [[l4 [ps4 [cs41 Heq4]]] [Hlcsim2 Hcssim2]]]]]]]; subst;
+  destruct HwfS1 as [Hinscope1' HwfECs'];
+  fold wf_ECStack in HwfECs';
+  unfold wf_ExecutionContext in Hinscope1';
+  simpl in Hinscope1'
+end.
+
+Lemma cmds_at_block_tail_next': forall l3 ps3 cs31 c cs tmn,
+  exists l1, exists ps1, exists cs11,
+         block_intro l3 ps3 (cs31 ++ c :: cs) tmn =
+         block_intro l1 ps1 (cs11 ++ cs) tmn.
+Proof.
+  intros.
+  exists l3. exists ps3. exists (cs31++[c]). simpl_env. auto.
+Qed.
+
+Definition pars_simulation (pinfo: PhiInfo) (lasinfo: LASInfo pinfo) (f1:fdef)
+  (ps1 ps2:params) : Prop :=
+  if (fdef_dec (PI_f pinfo) f1) then 
+    (List.map 
+      (fun p => 
+       let '(t, v):=p in 
+       (t, subst_value (LAS_lid pinfo lasinfo) (LAS_value pinfo lasinfo) v)) ps1)
+    = ps2
+  else ps1 = ps2.
+
+Lemma products_simulation__fdef_simulation : forall pinfo lasinfo Ps1 Ps2 fid f1 
+  f2,
+  lookupFdefViaIDFromProducts Ps2 fid = Some f2 ->
+  lookupFdefViaIDFromProducts Ps1 fid = Some f1 ->
+  products_simulation pinfo lasinfo Ps1 Ps2 ->
+  fdef_simulation pinfo lasinfo f1 f2.
+Admitted.
+
+Lemma lookupFdefViaPtr__simulation : forall pinfo lasinfo Ps1 Ps2 fptr f1 f2 fs,
+  OpsemAux.lookupFdefViaPtr Ps2 fs fptr = Some f2 ->
+  products_simulation pinfo lasinfo Ps1 Ps2 ->
+  OpsemAux.lookupFdefViaPtr Ps1 fs fptr = Some f1 ->
+  fdef_simulation pinfo lasinfo f1 f2.
+Proof.
+  intros.
+  unfold OpsemAux.lookupFdefViaPtr in *.
+  remember (OpsemAux.lookupFdefViaGVFromFunTable fs fptr) as R2.
+  destruct R2 as [fid|]; inv H1. simpl in H.
+  eapply products_simulation__fdef_simulation in H0; eauto.
+Qed.
+
+Lemma fdef_simulation__entry_block_simulation: forall pinfo lasinfo F1 F2 B1 B2,
+  fdef_simulation pinfo lasinfo F1 F2 ->
+  getEntryBlock F1 = ret B1 ->
+  getEntryBlock F2 = ret B2 ->
+  block_simulation pinfo lasinfo F1 B1 B2.
+Admitted.
+
+Lemma fdef_simulation_inv: forall pinfo lasinfo fh1 fh2 bs1 bs2,
+  fdef_simulation pinfo lasinfo (fdef_intro fh1 bs1) (fdef_intro fh2 bs2) ->
+  fh1 = fh2 /\ 
+  List.Forall2 
+    (fun b1 b2 => block_simulation pinfo lasinfo (fdef_intro fh1 bs1) b1 b2) 
+    bs1 bs2.
+Admitted.
+
+Lemma params2GVs_sim_aux : forall
+  (s : system) pinfo lasinfo 
+  los nts
+  (ps : list product)
+  (f : fdef)
+  (i0 : id)
+  n c t v p2
+  (cs : list cmd)
+  (tmn : terminator)
+  lc (gl : GVMap) ifs
+  (Hwfg1 : wf_global (los,nts) s gl)
+  (HwfF : wf_fdef ifs s (module_intro los nts ps) f)
+  (l1 : l)
+  (ps1 : phinodes)
+  (cs1 : list cmd)
+  (Hreach : isReachableFromEntry f
+             (block_intro l1 ps1 (cs1 ++ insn_call i0 n c t v p2 :: cs) tmn))
+  (HbInF : blockInFdefB
+            (block_intro l1 ps1 (cs1 ++ insn_call i0 n c t v p2 :: cs) tmn) f =
+          true)
+  (l0 : list atom)
+  (HeqR : ret l0 =
+         inscope_of_cmd f
+           (block_intro l1 ps1 (cs1 ++ insn_call i0 n c t v p2 :: cs) tmn)
+           (insn_call i0 n c t v p2))
+  (Hinscope : id_rhs_val.wf_defs (value_id (LAS_lid pinfo lasinfo)) 
+           (LAS_value pinfo lasinfo) (PI_f pinfo) (los, nts) gl f lc l0)
+  p22 p22' gvs gvs'
+  (Hex : exists p21, p2 = p21 ++ p22)
+  (Hp2gv : Opsem.params2GVs (los, nts) p22 lc gl = Some gvs)
+  (Hp2gv' : Opsem.params2GVs (los, nts) p22' lc gl = Some gvs')
+  (Hpasim : pars_simulation pinfo lasinfo f p22 p22'),
+  gvs = gvs'.
+Proof.
+(*
+  induction p22; intros; simpl; eauto.
+
+    destruct a as [[t0 attr0] v0].
+    destruct Hex as [p21 Hex]; subst.
+    assert (exists gv, getOperandValue (los, nts) v0 lc gl = Some gv)
+      as J.
+      eapply getOperandValue_inCmdOps_isnt_stuck; eauto.
+        simpl. unfold valueInParams. right. 
+        assert (J:=@in_split_r _ _ (p21 ++ (t0, attr0, v0) :: p22) 
+          (t0, attr0, v0)).
+        remember (split (p21 ++ (t0, attr0, v0) :: p22)) as R.
+        destruct R.
+        simpl in J. apply J.
+        apply In_middle.
+    destruct J as [gv J]. 
+    rewrite J.         
+    eapply IHp22 in HbInF; eauto.  
+      destruct HbInF as [vidxs HbInF].
+      rewrite HbInF. eauto.
+
+      exists (p21 ++ [(t0, attr0,v0)]). simpl_env. auto.
+Qed.
+*)
+Admitted.
+
+Lemma params2GVs_sim : forall
+  (s : system) pinfo lasinfo 
+  los nts
+  (ps : list product)
+  (f : fdef)
+  (i0 : id)
+  n c t v p2
+  (cs : list cmd)
+  (tmn : terminator)
+  lc (gl : GVMap) ifs
+  (Hwfg1 : wf_global (los,nts) s gl)
+  (HwfF : wf_fdef ifs s (module_intro los nts ps) f)
+  (l1 : l)
+  (ps1 : phinodes)
+  (cs1 : list cmd)
+  (Hreach : isReachableFromEntry f
+             (block_intro l1 ps1 (cs1 ++ insn_call i0 n c t v p2 :: cs) tmn))
+  (HbInF : blockInFdefB
+            (block_intro l1 ps1 (cs1 ++ insn_call i0 n c t v p2 :: cs) tmn) f =
+          true)
+  (l0 : list atom)
+  (HeqR : ret l0 =
+         inscope_of_cmd f
+           (block_intro l1 ps1 (cs1 ++ insn_call i0 n c t v p2 :: cs) tmn)
+           (insn_call i0 n c t v p2))
+  (Hinscope : id_rhs_val.wf_defs (value_id (LAS_lid pinfo lasinfo)) 
+           (LAS_value pinfo lasinfo) (PI_f pinfo) (los, nts) gl f lc l0)
+  p2' gvs gvs'
+  (Hp2gv : Opsem.params2GVs (los, nts) p2 lc gl = Some gvs)
+  (Hp2gv' : Opsem.params2GVs (los, nts) p2' lc gl = Some gvs')
+  (Hpasim : pars_simulation pinfo lasinfo f p2 p2'),
+  gvs = gvs'.
+Proof.
+  intros.
+  eapply params2GVs_sim_aux; eauto.
+    exists nil. auto.
+Qed.
+
+Lemma lookupFdefViaPtr__simulation_l2r : forall pinfo lasinfo Ps1 Ps2 fptr f1 fs,
+  products_simulation pinfo lasinfo Ps1 Ps2 ->
+  OpsemAux.lookupFdefViaPtr Ps1 fs fptr = Some f1 ->
+  exists f2, 
+    OpsemAux.lookupFdefViaPtr Ps2 fs fptr = Some f2 /\
+    fdef_simulation pinfo lasinfo f1 f2.
+Admitted.
+
+Lemma lookupExFdecViaPtr__simulation_l2r : forall pinfo lasinfo Ps1 Ps2 fptr f fs,
+  products_simulation pinfo lasinfo Ps1 Ps2 ->
+  OpsemAux.lookupExFdecViaPtr Ps1 fs fptr = Some f ->
+  OpsemAux.lookupExFdecViaPtr Ps2 fs fptr = Some f.
+Admitted.
+
 Lemma las_is_sim : forall pinfo lasinfo Cfg1 St1 Cfg2 St2 St2' tr2 tr1 St1'
   (Hwfpi: WF_PhiInfo pinfo) 
   (Hwfpp: OpsemPP.wf_State Cfg1 St1) 
+  (HwfS1: id_rhs_val.wf_State (value_id (LAS_lid pinfo lasinfo)) 
+           (LAS_value pinfo lasinfo) (PI_f pinfo) Cfg1 St1)
   (Hsim: State_simulation pinfo lasinfo Cfg1 St1 Cfg2 St2)
   (Hop2: Opsem.sInsn Cfg2 St2 St2' tr2) 
   (Hop1: Opsem.sInsn Cfg1 St1 St1' tr1), 
   State_simulation pinfo lasinfo Cfg1 St1' Cfg2 St2' /\ tr1 = tr2.
 Proof.
-(*
-  intros.
-  (sInsn_cases (induction Hop) Case).
-*)
 
-Admitted.
+Local Opaque inscope_of_tmn inscope_of_cmd.
+
+  intros.
+  (sInsn_cases (destruct Hop1) Case).
+
+Case "sReturn".
+
+  destruct_ctx_return.
+
+  assert (exists Result2,
+    tmn2 = insn_return rid RetTy Result2 /\ 
+    value_simulation pinfo lasinfo F Result Result2) as Hreturn.
+    clear - Htsim2.
+    unfold value_simulation, tmn_simulation in *.
+    destruct (fdef_dec (PI_f pinfo) F); inv Htsim2; eauto.
+  destruct Hreturn as [Result2 [EQ Hvsim2]]; subst.
+
+  inv Hop2.
+
+  match goal with
+  | H0 : free_allocas ?td ?M ?las = _,
+    H26 : free_allocas ?td ?M ?las = _ |- _ =>
+      rewrite H0 in H26; inv H26
+  end.
+  wfCall_inv.
+
+  assert (lc'' = lc''0) as EQ.
+    clear - H27 H1 Hcsim2' Hvsim2 Hinscope1' HwfSystem HmInS Hreach1 HBinF1 
+      HFinPs1 Hwfg.
+    unfold Opsem.returnUpdateLocals in H1, H27.
+    inv_mbind'.
+    destruct c1'; tinv H0.
+    assert (i0 = i1 /\ n = n0 /\ t0 = t) as EQ.
+      unfold cmd_simulation in Hcsim2';
+      destruct (fdef_dec (PI_f pinfo) F'); inv Hcsim2'; auto.
+    destruct EQ as [Heq1 [Heq2 Heq3]]; subst.
+    destruct n0; try solve [inv H0; inv H2; auto].
+    destruct t; tinv H0.
+    inv_mbind'.
+    remember (inscope_of_tmn F
+                   (block_intro l3 ps3 (cs3 ++ nil)
+                      (insn_return rid RetTy Result))
+                   (insn_return rid RetTy Result)) as R.
+    destruct R; tinv Hinscope1'.
+    symmetry_ctx.
+    eapply getOperandValue_inTmnOperands_sim in HeqR0; eauto
+      using wf_system__wf_fdef; simpl; auto.
+    subst. uniq_result. auto.
+    
+  subst.
+  repeat (split; eauto 2 using cmds_at_block_tail_next).
+
+Case "sReturnVoid".
+  destruct_ctx_return.
+
+  assert (tmn2 = insn_return_void rid) as Hreturn.
+    clear - Htsim2.
+    unfold value_simulation, tmn_simulation in *.
+    destruct (fdef_dec (PI_f pinfo) F); inv Htsim2; auto.
+  subst.
+
+  inv Hop2.
+
+  match goal with
+  | H0 : free_allocas ?td ?M ?las = _,
+    H26 : free_allocas ?td ?M ?las = _ |- _ =>
+      rewrite H0 in H26; inv H26
+  end.
+  wfCall_inv.
+  repeat (split; eauto 2 using cmds_at_block_tail_next).
+
+Case "sBranch".
+Focus.
+
+  destruct_ctx_other.
+  apply cmds_simulation_nil_inv in Hcssim2; subst.
+
+  assert (exists Cond2,
+    tmn2 = insn_br bid Cond2 l1 l2 /\ 
+    value_simulation pinfo lasinfo F Cond Cond2) as Hbr.
+    clear - Htsim2.
+    unfold value_simulation, tmn_simulation in *.
+    destruct (fdef_dec (PI_f pinfo) F); inv Htsim2; eauto.
+  destruct Hbr as [Cond2 [EQ Hvsim2]]; subst.
+
+  inv Hop2.
+  uniq_result.
+  remember (inscope_of_tmn F (block_intro l3 ps3 (cs31 ++ nil) 
+             (insn_br bid Cond l1 l2)) (insn_br bid Cond l1 l2)) as R.
+  destruct R; tinv Hinscope1'.
+
+  assert (uniqFdef F) as HuniqF.
+    eauto using wf_system__uniqFdef.
+  assert (wf_fdef nil S (module_intro los nts Ps) F) as HwfF.
+    eauto using wf_system__wf_fdef.
+  assert (c = c0)as Heq.
+    eapply getOperandValue_inTmnOperands_sim with (v:=Cond)(v':=Cond2); 
+      try solve [eauto | simpl; auto].
+  subst.
+  assert (block_simulation pinfo lasinfo F 
+           (block_intro l' ps' cs' tmn')
+           (block_intro l'0 ps'0 cs'0 tmn'0)) as Hbsim.
+    clear - H22 H1 Hfsim2.
+    destruct (isGVZero (los, nts) c0); eauto using fdef_sim__block_sim.
+  assert (Hbsim':=Hbsim).
+  apply block_simulation_inv in Hbsim'.
+  destruct Hbsim' as [Heq [Hpsim' [Hcssim' Htsim']]]; subst.
+
+  assert (isReachableFromEntry F (block_intro l'0 ps' cs' tmn') /\
+    In l'0 (successors_terminator (insn_br bid Cond l1 l2)) /\
+    blockInFdefB (block_intro l'0 ps' cs' tmn') F = true) as J.
+    symmetry in H1.
+    destruct (isGVZero (los,nts) c0);
+      assert (J:=H1);
+      apply lookupBlockViaLabelFromFdef_inv in J; eauto;
+      destruct J as [J H13']; subst;
+      (repeat split; simpl; auto); try solve [
+        auto | eapply reachable_successors; (eauto || simpl; auto)].
+  destruct J as [Hreach' [Hsucc' HBinF1']].
+
+  assert (lc' = lc'0) as Heq.
+    eapply switchToNewBasicBlock_sim in Hbsim; eauto.
+  subst.
+  repeat (split; auto).
+    exists l'0. exists ps'. exists nil. auto.
+    exists l'0. exists ps'0. exists nil. auto.
+
+Unfocus.
+
+Case "sBranch_uncond".
+Focus.
+
+  destruct_ctx_other.
+  apply cmds_simulation_nil_inv in Hcssim2; subst.
+
+  assert (tmn2 = insn_br_uncond bid l0) as Hbr.
+    clear - Htsim2.
+    unfold value_simulation, tmn_simulation in *.
+    destruct (fdef_dec (PI_f pinfo) F); inv Htsim2; eauto.
+  subst.
+
+  inv Hop2.
+  uniq_result.
+  remember (inscope_of_tmn F (block_intro l3 ps3 (cs31 ++ nil) 
+             (insn_br_uncond bid l0)) (insn_br_uncond bid l0)) as R.
+  destruct R; tinv Hinscope1'.
+
+  assert (uniqFdef F) as HuniqF.
+    eauto using wf_system__uniqFdef.
+  assert (wf_fdef nil S (module_intro los nts Ps) F) as HwfF.
+    eauto using wf_system__wf_fdef.
+
+  assert (block_simulation pinfo lasinfo F 
+           (block_intro l' ps' cs' tmn')
+           (block_intro l'0 ps'0 cs'0 tmn'0)) as Hbsim.
+    clear - H H16 Hfsim2.
+    eauto using fdef_sim__block_sim.
+  assert (Hbsim':=Hbsim).
+  apply block_simulation_inv in Hbsim'.
+  destruct Hbsim' as [Heq [Hpsim' [Hcssim' Htsim']]]; subst.
+
+  assert (isReachableFromEntry F (block_intro l'0 ps' cs' tmn') /\
+    In l'0 (successors_terminator (insn_br_uncond bid l0)) /\
+    blockInFdefB (block_intro l'0 ps' cs' tmn') F = true) as J.
+    symmetry in H;
+    assert (J:=H);
+    apply lookupBlockViaLabelFromFdef_inv in J; eauto;
+    destruct J as [J H13']; subst;
+    (repeat split; simpl; auto); try solve [
+      auto | eapply reachable_successors; (eauto || simpl; auto)].
+  destruct J as [Hreach' [Hsucc' HBinF1']].
+
+  assert (lc' = lc'0) as Heq.
+    eapply switchToNewBasicBlock_sim in Hbsim; eauto.
+  subst.
+  repeat (split; auto).
+    exists l'0. exists ps'. exists nil. auto.
+    exists l'0. exists ps'0. exists nil. auto.
+
+Unfocus.
+
+Case "sBop".
+
+  destruct_ctx_other.
+  apply cmds_simulation_cons_inv in Hcssim2.
+  destruct Hcssim2 as [c1' [cs3' [Heq [Hcsim2 Hcssim2]]]]; subst.
+
+  assert (exists v1', exists v2',
+    c1' = insn_bop id0 bop0 sz0 v1' v2' /\ 
+    value_simulation pinfo lasinfo F v1 v1' /\
+    value_simulation pinfo lasinfo F v2 v2') as Hcmd.
+    clear - Hcsim2.
+    unfold value_simulation, cmd_simulation in *.
+    destruct (fdef_dec (PI_f pinfo) F); inv Hcsim2; eauto.
+  destruct Hcmd as [v1' [v2' [Heq [Hvsim1 Hvsim2]]]]; subst.
+  inv Hop2.
+
+  assert (wf_fdef nil S (module_intro los nts Ps) F) as HwfF.
+    eauto using wf_system__wf_fdef.
+
+  assert (gvs0 = gvs3) as Heq.
+    unfold Opsem.BOP in *.
+    inv_mbind'; inv_mfalse; app_inv; symmetry_ctx.
+
+    match goal with
+    | HeqR : Opsem.getOperandValue _ ?v1 _ _ = ret _, 
+      HeqR' : Opsem.getOperandValue _ ?v1' _ _ = ret _, 
+      HeqR0 : Opsem.getOperandValue _ ?v2 _ _ = ret _,
+      HeqR0' : Opsem.getOperandValue _ ?v2' _ _ = ret _,
+      Hvsim1 : value_simulation _ _ _ ?v1 ?v1',
+      Hvsim2 : value_simulation _ _ _ ?v2 ?v2' |- _ => 
+      eapply getOperandValue_inCmdOperands_sim with (v':=v1') in HeqR; 
+        try (eauto || simpl; auto);
+      eapply getOperandValue_inCmdOperands_sim with (v':=v2') in HeqR0; 
+        try (eauto || simpl; auto);
+      subst; uniq_result; auto
+    end.
+
+  subst.
+
+  repeat (split; eauto 2 using cmds_at_block_tail_next').
+
+Case "sFBop". admit.
+Case "sExtractValue". admit.
+Case "sInsertValue". admit.
+Case "sMalloc". 
+
+  destruct_ctx_other.
+  apply cmds_simulation_cons_inv in Hcssim2.
+  destruct Hcssim2 as [c1' [cs3' [Heq [Hcsim2 Hcssim2]]]]; subst.
+
+  assert (exists v',
+    c1' = insn_malloc id0 t v' align0 /\ 
+    value_simulation pinfo lasinfo F v v') as Hcmd.
+    clear - Hcsim2.
+    unfold value_simulation, cmd_simulation in *.
+    destruct (fdef_dec (PI_f pinfo) F); inv Hcsim2; eauto.
+  destruct Hcmd as [v' [Heq Hvsim]]; subst.
+  inv Hop2.
+
+  assert (wf_fdef nil S (module_intro los nts Ps) F) as HwfF.
+    eauto using wf_system__wf_fdef.
+
+  assert (gns = gns0) as Heq.
+    inv_mfalse; symmetry_ctx.
+    eapply getOperandValue_inCmdOperands_sim with (v':=v') in H0; 
+      try (eauto || simpl; auto).
+  subst.
+  uniq_result.
+  repeat (split; eauto 2 using cmds_at_block_tail_next').
+
+Case "sFree". admit.
+Case "sAlloca". admit.
+Case "sLoad". admit.
+Case "sStore". admit.
+Case "sGEP". admit.
+Case "sTrunc". admit.
+Case "sExt". admit.
+Case "sCast". admit.
+Case "sIcmp". admit.
+Case "sFcmp". admit.
+Case "sSelect". admit.
+Case "sCall".
+
+  destruct_ctx_other.
+  assert (Hcssim2':=Hcssim2).
+  apply cmds_simulation_cons_inv in Hcssim2.
+  destruct Hcssim2 as [c1' [cs3' [Heq [Hcsim2 Hcssim2]]]]; subst.
+
+  assert (exists fv', exists lp',
+    c1' = insn_call rid noret0 ca ft fv' lp' /\ 
+    value_simulation pinfo lasinfo F fv fv' /\
+    pars_simulation pinfo lasinfo F lp lp') as Hcmd.
+    clear - Hcsim2.
+    unfold value_simulation, cmd_simulation, pars_simulation in *.
+    destruct (fdef_dec (PI_f pinfo) F); inv Hcsim2; eauto.
+  destruct Hcmd as [fv' [lp' [Heq [Hvsim Hpasim]]]]; subst.
+
+  assert (wf_fdef nil S (module_intro los nts Ps) F) as HwfF.
+    eauto using wf_system__wf_fdef.
+
+  inv Hop2.
+
+  SCase "SCall".
+
+  uniq_result.
+
+  assert (fptr = fptr0) as Heq.
+    inv_mfalse; symmetry_ctx.
+    eapply getOperandValue_inCmdOperands_sim with (v':=fv') in H; 
+      try (eauto || simpl; auto).
+  subst. clear H.
+
+  assert (Hfsim1:=Hpsim).
+  eapply lookupFdefViaPtr__simulation in Hfsim1; eauto.
+
+  assert (Hbsim1:=Hfsim1).
+  eapply fdef_simulation__entry_block_simulation in Hbsim1; eauto.
+  assert (Hbsim1':=Hbsim1).
+  apply block_simulation_inv in Hbsim1'.
+  destruct Hbsim1' as [Heq' [Hpsim1' [Hcsim1' Htsim1']]]; subst.
+  repeat (split; eauto 4).
+    exists l'0. exists ps'. exists nil. auto.
+    exists l'0. exists ps'0. exists nil. auto.
+
+    assert (gvs = gvs0) as EQ.
+      inv_mfalse; symmetry_ctx.
+      eapply params2GVs_sim; eauto.
+    subst.
+    clear - H4 H31 Hfsim1.
+    apply fdef_simulation_inv in Hfsim1.
+    destruct Hfsim1 as [Heq _]. inv Heq. uniq_result.
+    auto.
+
+  SCase "sExCall".
+
+  uniq_result.
+
+  assert (fptr = fptr0) as Heq.
+    inv_mfalse; symmetry_ctx.
+    eapply getOperandValue_inCmdOperands_sim with (v':=fv') in H; 
+      try (eauto || simpl; auto).
+  subst. clear H.
+  clear - H28 H1 Hpsim.
+
+  eapply lookupFdefViaPtr__simulation_l2r in H1; eauto.
+  destruct H1 as [f2 [H1 H2]].
+  apply OpsemAux.lookupExFdecViaPtr_inversion in H28.
+  apply OpsemAux.lookupFdefViaPtr_inversion in H1.
+  destruct H28 as [fn [J1 [J2 J3]]].
+  destruct H1 as [fn' [J4 J5]].
+  uniq_result.   
+
+Case "sExCall". 
+
+  destruct_ctx_other.
+  assert (Hcssim2':=Hcssim2).
+  apply cmds_simulation_cons_inv in Hcssim2.
+  destruct Hcssim2 as [c1' [cs3' [Heq [Hcsim2 Hcssim2]]]]; subst.
+
+  assert (exists fv', exists lp',
+    c1' = insn_call rid noret0 ca ft fv' lp' /\ 
+    value_simulation pinfo lasinfo F fv fv' /\
+    pars_simulation pinfo lasinfo F lp lp') as Hcmd.
+    clear - Hcsim2.
+    unfold value_simulation, cmd_simulation, pars_simulation in *.
+    destruct (fdef_dec (PI_f pinfo) F); inv Hcsim2; eauto.
+  destruct Hcmd as [fv' [lp' [Heq [Hvsim Hpasim]]]]; subst.
+
+  assert (wf_fdef nil S (module_intro los nts Ps) F) as HwfF.
+    eauto using wf_system__wf_fdef.
+
+  inv Hop2.
+
+  SCase "SCall".
+
+  uniq_result.
+
+  assert (fptr = fptr0) as Heq.
+    inv_mfalse; symmetry_ctx.
+    eapply getOperandValue_inCmdOperands_sim with (v':=fv') in H; 
+      try (eauto || simpl; auto).
+  subst. clear H.
+  clear - H29 H1 Hpsim.
+
+  eapply lookupExFdecViaPtr__simulation_l2r in H1; eauto.
+  apply OpsemAux.lookupExFdecViaPtr_inversion in H1.
+  apply OpsemAux.lookupFdefViaPtr_inversion in H29.
+  destruct H1 as [fn [J1 [J2 J3]]].
+  destruct H29 as [fn' [J4 J5]].
+  uniq_result.   
+
+  SCase "sExCall".
+
+  uniq_result.
+
+  assert (fptr = fptr0) as Heq.
+    inv_mfalse; symmetry_ctx.
+    eapply getOperandValue_inCmdOperands_sim with (v':=fv') in H; 
+      try (eauto || simpl; auto).
+  subst. clear H.
+
+  assert (Hlkdec:=Hpsim).
+  eapply lookupExFdecViaPtr__simulation_l2r in Hlkdec; eauto.
+
+  assert (gvss = gvss0) as EQ.
+    inv_mfalse; symmetry_ctx.
+    eapply params2GVs_sim; eauto.
+  subst.
+  uniq_result.
+
+  repeat (split; eauto 2 using cmds_at_block_tail_next').
+
+Transparent inscope_of_tmn inscope_of_cmd.
+
+Qed.
+
 
 (*****************************)
 (*
